Added equivalence proofs for redc_alt, a version of redc done using fold

src/Arithmetic/WordByWordMontgomery.v
@@ -128,13 +128,94 @@ Module WordByWordMontgomery.
 
       (*Nathan nonsense begins here*)
 
+      Definition pre_redc_from (S': T (S R_numlimbs)) : T (S R_numlimbs)
+        := snd (redc_loop A_numlimbs (A, S')).
+      
       Definition redc_body_alt: Z * T (S R_numlimbs) -> T (S R_numlimbs)
         := fun '(a, S') => a'_S3 B k S' a.
 
+      Definition redc_loop_alt: T (S R_numlimbs) :=
+        fold_left (fun S a => redc_body_alt (a, S)) A (@zero (1 + R_numlimbs)%nat).
+
+      Definition redc_loop_alt_from (S': T (S R_numlimbs)) : T (S R_numlimbs) :=
+        fold_left (fun S a => redc_body_alt (a, S)) A S'.
+
+      Definition redc_alt: T (R_numlimbs) :=
+        conditional_sub redc_loop_alt N.
+
+      (*
+      Fixpoint atIndex {len: nat} (l : T len) (index : nat) : Z :=
+        match len with
+        | O => 0
+        | S len' =>
+            match index with
+            | O => snd (@divmod len' l)
+            | S pred_index => atIndex (fst (@divmod len' l)) pred_index
+            end
+        end.
+      
+      Fixpoint redc_loop_alt' (count: nat) : T (S R_numlimbs) :=
+        match count with
+        |O => @zero (1 + R_numlimbs)%nat
+        |S pred_count => redc_body_alt (atIndex A (count - 1), redc_loop_alt pred_count)
+        end.
+
+      Definition redc_alt' : T (R_numlimbs) :=
+        conditional_sub (redc_loop_alt A_numlimbs) N.
+       *)
+      
       (*Nathan nonsense ends here*)
-          
     End loop.
+
+    Lemma redc_loop_alt_from_eq:
+      forall {A_numlimbs: nat} (A: T A_numlimbs) (B: T R_numlimbs) (k: Z) (S_old: T (S R_numlimbs)),
+        redc_loop_alt_from (length A) A B k S_old = pre_redc_from (length A) A B k S_old.
+      Proof. 
+        intros. generalize dependent S_old. induction A.
+        - reflexivity.
+        - intros.
+          cbv [pre_redc_from redc_loop_alt_from]. simpl. cbv [redc_loop_alt_from redc_body_alt] in IHA.  rewrite IHA.
+          cbv [pre_redc_from]. f_equal.
+      Qed.
+
+      Lemma pre_redc_from_zero:
+        forall {A_numlimbs: nat} (A: T A_numlimbs) (B: T R_numlimbs) (k: Z),
+          pre_redc (length A) A B k = pre_redc_from (length A) A B k zero.
+      Proof.
+        intros. reflexivity.
+      Qed.
+
+      Lemma redc_loop_alt_from_zero:
+        forall {A_numlimbs: nat} (A: T A_numlimbs) (B: T R_numlimbs) (k: Z),
+          redc_loop_alt (length A) A B k = redc_loop_alt_from (length A) A B k zero.
+      Proof.
+        intros. reflexivity.
+      Qed.
+      
+    Theorem redc_alt_eq:
+      forall {A_numlimbs: nat} (A: T A_numlimbs) (B: T R_numlimbs) (k : Z),
+        redc (length A) A B k = redc_alt (length A) A B k.
+    Proof.
+      intros. cbv [redc redc_alt]. f_equal. rewrite pre_redc_from_zero. rewrite redc_loop_alt_from_zero.
+      symmetry. apply redc_loop_alt_from_eq.
+    Qed.
     
+    
+    (*
+    Example redc_alt'_eq_3:  forall (A : T _) (B : T R_numlimbs) (k : Z),
+        redc 3 A B k = redc_alt' 3 A B k.
+    Proof. intros. reflexivity. Qed.
+    
+    Theorem redc_alt'_eq:
+        forall (count : nat) (A : T _) (B : T R_numlimbs) (k : Z),
+        redc count A B k = redc_alt' count A B k.
+    Proof.
+      intros. cbv [redc redc_alt pre_redc redc_alt']. f_equal.
+      induction count as [|count' IHcount].
+      - reflexivity. 
+      - simpl. rewrite Nat.sub_diag. Abort.
+      *)
+
 
     Create HintDb word_by_word_montgomery.
     Hint Unfold A'_S3 S3' S2 q s S1 a A' A_a Let_In : word_by_word_montgomery.
